Important chage!! Use Linear IR instead of of Mach. Previous proof was renamed into Schedulinproof_old.v . The proof structure are very simillar but more simple

backend/Schedulingproof.v
@@ -14,9 +14,7 @@ End SMALL_STEP_EXT.
 
 
 Require Import Coqlib Maps BoolEqual.
-Require Import AST Integers Values Events Memory Linking Globalenvs Smallstep.
-Require Import Op Locations Conventions Machregs.
-Require Import Mach Asmgenproof0 Asmgenproof.
+
 
 Import ListNotations.
 Open Scope list_scope. 
@@ -36,9 +34,9 @@ Section TOPO.
     | Datatypes.S n', i :: l' => i :: try_swap n' l'
     end. 
   
-  Lemma try_swap_later: 
+  (* Lemma try_swap_later: 
     forall (n:nat) l a, 0 < n -> try_swap n (a :: l) = a :: try_swap (n-1) l.
-  Proof. Admitted.
+  Proof. Admitted. *)
 
   Lemma try_swap_nil: forall n, try_swap n [] = [].
   Proof. intros; destruct n; auto. Qed.
@@ -76,11 +74,16 @@ Section TOPO.
   End DECIDE_REL.
 End TOPO.
 
-
 Require Import Errors.
+Require Import AST Integers Values Events Memory Linking Globalenvs Smallstep.
+Require Import Op Locations Conventions Machregs.
+Require Import Linear Asmgenproof0 Asmgenproof.
+
+
 Open Scope error_monad_scope.
 Import ListNotations.
 Open Scope list_scope.
+
 Section SIMULATION_SEQUENCE.
   Definition transf_program_one (transf_def: ident -> fundef -> fundef) :=
       transform_partial_program2 
@@ -95,18 +98,12 @@ Section SIMULATION_SEQUENCE.
         transf_program_sequence tfl' p'
     end.
 
-  Variable return_address_offset: function -> code -> ptrofs -> Prop.
-  (* Variable funid: ident. *)
-  
   Definition transf_single_fun_fsim_preserve (transf_def: ident -> fundef -> fundef):=
     forall prog tprog, 
-    (* let transf_fun := (fun i f => if ident_eq i funid then transf_def f else OK f) in
-    let transf_var := (fun (i: ident) (v:unit) => OK v) in *)
     transform_partial_program2 
-      (fun i f => OK (transf_def i f)) 
-      (fun i v => OK v) prog = OK tprog ->
-    forward_simulation (Mach.semantics return_address_offset prog) 
-    (Mach.semantics return_address_offset tprog).
+      (fun i f => OK (transf_def i f)) (fun i v => OK v) prog = OK tprog ->
+    forward_simulation (Linear.semantics prog) 
+    (Linear.semantics tprog).
 
   Definition transf_fundef_list_preserved(lf: list (ident -> fundef -> fundef)): Prop :=
     Forall transf_single_fun_fsim_preserve lf.
@@ -118,8 +115,8 @@ Section SIMULATION_SEQUENCE.
   Hypothesis TRANSF_PROG: transf_program_sequence tfl prog = OK tprog.
   
   Theorem forward_simulation_sequence:
-    forward_simulation (Mach.semantics return_address_offset prog) 
-                       (Mach.semantics return_address_offset tprog).
+    forward_simulation (Linear.semantics prog) 
+                       (Linear.semantics tprog).
   Proof.
     revert prog tprog TRANSF_PROG.
     induction safe_list; intros.
@@ -127,19 +124,13 @@ Section SIMULATION_SEQUENCE.
     - inv safe_list. specialize (IHt H3).
       simpl in TRANSF_PROG. monadInv TRANSF_PROG. rename x0 into tmprog.
       eapply compose_forward_simulations 
-        with (L2:= semantics return_address_offset tmprog); auto.
+        with (L2:= semantics tmprog); auto.
   Qed.
 
   (* Definition real_match_prog (prog tprog: program) :=
     match_program (fun ctx f tf => real_transf_fundef f = OK tf) eq prog tprog. *)
 
 End SIMULATION_SEQUENCE.
-
-Check forward_simulation_sequence.
-
-Section SIMULATION_FRAMEWORK.
-  
-End SIMULATION_FRAMEWORK.
 
 (** [i1: reg = ...] :: [i2: ... = op args] :: [...] *)
 Fixpoint mregs_in_list (args: list mreg) (reg: mreg):=
@@ -151,35 +142,35 @@ Fixpoint mregs_in_list (args: list mreg) (reg: mreg):=
 
 Definition solid_inst (i: instruction): bool :=
     match i with
-    | Mgetparam _ _ _ => true  (* TODO: is this fine? *)
-    | Mcall _ _  | Mtailcall _ _  | Mbuiltin _ _ _ 
-    | Mlabel _  | Mgoto _ | Mcond _ _ _ | Mjumptable _ _
-    | Mreturn => true
+    | Lcall _ _  | Ltailcall _ _  | Lbuiltin _ _ _ 
+    | Llabel _  | Lgoto _ | Lcond _ _ _ | Ljumptable _ _
+    | Lreturn => true
     | _ => false
     end.
 
 (* Some true: memory write, Some false: memory read. None: no memory operation *)
+(* Note: when linear was transformed to Mach, set/get stack inst. will access memory,
+    though it is seperate *)
 Definition mem_write (i: instruction): option bool :=
     match i with
-    | Mgetstack _ _ _ => Some false
-    | Msetstack _ _ _ => Some true
-    | Mload _ _ _ dst => Some false
-    | Mstore _ _ _ src => Some true
+    | Lgetstack _ _ _ _ => Some false
+    | Lsetstack _ _ _ _ => Some true
+    | Lload _ _ _ dst => Some false
+    | Lstore _ _ _ src => Some true
     | _ => None
     end. 
 
-(* (src register, false:read/true:write/None mem) *)
 Definition get_dst (i: instruction): option mreg :=
     match i with
-    | Mgetstack _ _ dst | Mgetparam _ _ dst
-    | Mop _ _ dst | Mload _ _ _ dst => Some dst
+    | Lgetstack _ _ _ dst
+    | Lop _ _ dst | Lload _ _ _ dst => Some dst
     | _ => None
     end. 
 
 Definition get_srcs (i: instruction): list mreg :=
     match i with
-    | Mop op args res => args
-    | Msetstack src _ _  | Mstore _ _ _ src => src::nil
+    | Lop op args res => args
+    | Lsetstack src _ _ _  | Lstore _ _ _ src => src::nil
     | _ => nil
     end. 
 
@@ -227,18 +218,11 @@ Definition happens_before (i1 i2: instruction): bool :=
 
 Notation "i1 D~> i2":= (happens_before i1 i2) (at level 1).
 
-(** topo order from deta independence *)
-Parameter GraphType: Type.
-Fixpoint topo_calcu (bb: list instruction): GraphType. Admitted.
-
-(** swap some pair of consecutive inst. in code *)
-(* note that those are not actual functions that will be used in compiling, but only in correctness proof *)
 
 Definition try_swap_code:= try_swap happens_before.
 
 Definition try_swap_nth_func (n: nat)(f: function):= 
-    mkfunction f.(fn_sig) (try_swap_code n f.(fn_code)) 
-               f.(fn_stacksize) f.(fn_link_ofs) f.(fn_retaddr_ofs).
+    mkfunction f.(fn_sig) f.(fn_stacksize) (try_swap_code n f.(fn_code)) .
 
 Definition transf_function_try_swap_nth (n: nat) (f: function) : res function :=
     OK (try_swap_nth_func n f).
@@ -252,181 +236,29 @@ Definition transf_program_try_swap_nth_in_one (funid: ident) (n: nat) (p: progra
   (fun i f => if ident_eq i funid then transf_fundef_try_swap_nth n f else OK f) 
   (fun i v => OK v) p.
 
-(* Fixpoint transf_program_try_swap_multi_in_one (funid: ident) (ln: list nat)(p: program): res program :=
-  match ln with
-  | nil => OK p
-  | n :: ln' => do p' <- transf_program_try_swap_nth_in_one funid n p;
-                transf_program_try_swap_multi_in_one funid ln' p'
-  end. *)
 
-(* Fixpoint transf_program_try_swap_multi_in_multi (pairs:list (ident * list nat))(p:program): res program:=
-  match pairs with
-  | nil => OK p
-  | (funid, ln) :: pairs' => 
-    do p' <- transf_program_try_swap_multi_in_one funid ln p;
-    transf_program_try_swap_multi_in_multi pairs' p  
-  end. *)
 
-(** Extension from Globleenvs.v *)
-(* Section GENV_EXT.
-    Section TRANSF_PROGRAM_EXT.
+Section LOCSET_AGREE.
 
-    Context {A B V W: Type}.
-    Variable transf_fun: ident -> A -> B.
-    Variable transf_var: ident -> V -> res W.
+  Definition lsagree (rs rs': locset) := 
+    forall r: loc, Locmap.get r rs = Locmap.get r rs'.
 
-    Definition transf_globdef (idg: ident * globdef A V) : ident * globdef B V :=
-        match idg with
-        | (id, Gfun f) => (id, Gfun (transf_fun id f))
-        | (id, Gvar v) => (id, Gvar v)
-        end.
-
-    End TRANSF_PROGRAM_EXT.
-End GENV_EXT. *)
-
-(* Machting relation between register relations *)
-Section RS_AGREE.
-  Definition rsagree (rs rs': regset) := 
-    forall r:mreg, Regmap.get r rs = Regmap.get r rs'. 
-
-  Lemma rsagree_symmetric: symmetric _ rsagree.
+  Lemma lsagree_refl: reflexive _ lsagree.
   Proof. hnf; intros; intro; auto. Qed.
 
-  Lemma rsagree_inv_swap: 
-    forall rs rs', rsagree rs rs' -> 
-      forall ra va rb vb, ra <> rb ->
-        rsagree (rs # ra <- va # rb <- vb) (rs' # rb <- vb # ra <- va).
-  Proof.
-    intros; intro. unfold Regmap.get, Regmap.set.
-    destruct (RegEq.eq r ra); destruct (RegEq.eq r rb); subst; simpl; auto.
-    - destruct H0; auto. - apply H. 
-  Qed.
-
-  Lemma rsagree_inv_update:
-    forall rs rs', rsagree rs rs' -> 
-      forall r v, rsagree (rs # r <- v) (rs' # r <- v).
-  Proof. 
-    intros; intro; unfold Regmap.get, Regmap.set.
-    destruct RegEq.eq; auto. eapply H.
-  Qed.
-
-  Lemma rsagree_inv_mreg_list:
-    forall lr rs rs', rsagree rs rs' ->
-      rs ## lr = rs' ## lr.
-  Proof. 
-    intros lr. induction lr; simpl; auto; intros. specialize (IHlr _ _ H). 
-    rewrite <- IHlr. assert (rs a = rs' a). apply H. rewrite H0; auto. 
-  Qed.
-
-  Lemma rsagree_inv_undef_regs_destroyed:
-    forall lr rs rs', rsagree rs rs' ->
-      rsagree (undef_regs lr rs)
-              (undef_regs lr rs').
-  Proof. 
-    intros lr. induction lr; intros; simpl; auto.
-    intro. unfold Regmap.get, Regmap.set. destruct (RegEq.eq r a); simpl; auto.
-    apply IHlr; auto.
-  Qed.
-
-  Lemma rsagree_inv_extcall_arg:
-    forall rs rs' m sp l v, 
-        rsagree rs rs' -> extcall_arg rs m sp l v ->
-        extcall_arg rs' m sp l v.
-  Proof. 
-    intros. inv H0.
-    - unfold rsagree, Regmap.get in H; rewrite H. eapply extcall_arg_reg.
-    - eapply extcall_arg_stack; eauto.
-  Qed.
-
-  Lemma rsagree_inv_extcall_arg_pair:
-    forall rs rs' m sp l v, 
-      rsagree rs rs' -> extcall_arg_pair rs m sp l v ->
-      extcall_arg_pair rs' m sp l v.
-  Proof.
-    intros. inv H0.
-    - eapply extcall_arg_one. eapply rsagree_inv_extcall_arg; eauto.
-    - eapply extcall_arg_twolong; eapply rsagree_inv_extcall_arg; eauto.
-  Qed.
-
-  Lemma rsagree_inv_extcall_arguments: 
-    forall args rs rs' m sp sg , 
-      rsagree rs rs' -> extcall_arguments rs m sp sg args ->
-        extcall_arguments rs' m sp sg args.
-  Proof. 
-    intros. hnf in *.
-    eapply list_forall2_imply. eapply H0. intros.
-    eapply rsagree_inv_extcall_arg_pair; eauto.
-  Qed.
-
-  Lemma rsagree_inv_eval_builtin_arg:
-    forall ge rs rs' sp m arg var,
-    rsagree rs rs' -> eval_builtin_arg ge rs sp m arg var -> 
-      eval_builtin_arg ge rs' sp m arg var.
-  Proof. 
-    intros. unfold rsagree, Regmap.get in H. induction H0; try rewrite H.
-    - apply eval_BA. - apply eval_BA_int. - apply eval_BA_long.
-    - apply eval_BA_float. - apply eval_BA_single.
-    - apply eval_BA_loadstack; auto. - apply eval_BA_addrstack.
-    - apply eval_BA_loadglobal; auto. - apply eval_BA_addrglobal.
-    - apply eval_BA_splitlong; auto. - apply eval_BA_addptr; auto.
-  Qed.
-
-  Lemma rsagree_inv_eval_builtin_args:
-    forall ge rs rs' sp m args vargs,
-    rsagree rs rs' -> eval_builtin_args ge rs sp m args vargs -> 
-      eval_builtin_args ge rs' sp m args vargs.
-  Proof. 
-    intros. hnf in *. Check list_forall2_imply.
-    eapply list_forall2_imply. eapply H0. intros; auto. 
-    eapply rsagree_inv_eval_builtin_arg; eauto.
-  Qed.
-
-  Lemma rsagree_inv_undef_caller_save_regs:
-    forall rs rs', rsagree rs rs' ->
-      rsagree (undef_caller_save_regs rs) (undef_caller_save_regs rs').
-  Proof.
-    intros; intro. unfold Regmap.get, undef_caller_save_regs.
-    destruct is_callee_save; auto. apply H.
-  Qed.
-
-  Lemma rsagree_inv_set_pair:
-    forall rs rs' p res, rsagree rs rs' ->
-      rsagree (set_pair p res rs) (set_pair p res rs').
-  Proof.
-    intros; intro. unfold Regmap.get. destruct p; simpl.
-    unfold Regmap.set; destruct (RegEq.eq r r0); simpl; eauto.
-    unfold Regmap.set; destruct (RegEq.eq r rlo); destruct (RegEq.eq r rhi); simpl; eauto.
-  Qed.
-
-  Lemma rsagree_inv_set_res:
-    forall res v rs rs', rsagree rs rs' ->
-      rsagree (set_res res v rs) (set_res res v rs'). 
-  Proof. 
-    intros res. unfold Regmap.get. induction res; simpl; auto; intros.
-    - apply rsagree_inv_update; auto.
-  Qed. 
-
-  Lemma rsagree_inv_find_function_ptr:
-    forall ge ros rs rs', rsagree rs rs' ->
-      find_function_ptr ge ros rs = find_function_ptr ge ros rs'.
-  Proof. 
-    intros. destruct ros; auto. 
-    simpl. unfold rsagree, Regmap.get in H. rewrite H; auto.
-  Qed.
+  Lemma lsagree_symmetric: symmetric _ lsagree.
+  Proof. hnf; intros; intro; auto. Qed.
 
 
-  (* Lemma rsagree_inv_eval_condition: 
-    forall cond args m rs rs', rsagree rs rs' ->
-      eval_condition cond rs ## args m = eval_condition cond rs' ## args m.
-  Proof. intros. Locate "##". Check eval_condition. Print map. Locate map. *)
 
-End RS_AGREE.
+End LOCSET_AGREE.
 
-Lemma find_function_ptr_genv_irrelevent:
+
+(* Lemma find_function_ptr_genv_irrelevent:
   forall ge1 ge2 ros rs,
     (forall (s: ident), Genv.find_symbol ge1 s = Genv.find_symbol ge2 s) ->
       find_function_ptr ge1 ros rs = find_function_ptr ge2 ros rs.
-Proof. intros. destruct ros; auto; simpl. apply H. Qed.
+Proof. intros. destruct ros; auto; simpl. apply H. Qed. *)
 
 Lemma extcall_genv_irrelevent:
   forall ge1 ge2 ef args m1 t res m2,
@@ -449,15 +281,15 @@ Qed.
 
 Section FIND_LABEL.
 
-Lemma is_label_inv: forall lbl a, is_label lbl a = true -> a =  Mlabel lbl.
+Lemma is_label_inv: forall lbl a, is_label lbl a = true -> a =  Llabel lbl.
 Proof. 
   intros. destruct a; simpl in H; inv H. destruct (peq lbl l). 
   rewrite e; auto. discriminate H1. 
 Qed.
 
 Lemma find_label_try_swap:
-  forall lbl c c' n, Mach.find_label lbl c = Some c' ->
-    exists n', Mach.find_label lbl (try_swap_code n c) = Some (try_swap_code n' c').
+  forall lbl c c' n, Linear.find_label lbl c = Some c' ->
+    exists n', Linear.find_label lbl (try_swap_code n c) = Some (try_swap_code n' c').
 Proof.
   intros lbl c. revert lbl. induction c; intros.
   - exists O. inv H.
@@ -485,12 +317,61 @@ Qed.
 
 End FIND_LABEL.
 
+
+Lemma Linear_determ: forall p, determinate (Linear.semantics p).
+  Proof. 
+    constructor.
+    - intros. inv H; inv H0.
+      + split. eapply match_traces_E0. intros; auto.
+      + split. eapply match_traces_E0. intros; auto.
+      + split. eapply match_traces_E0. intros; auto. rewrite H12 in H1; inv H1; auto.
+      + split. eapply match_traces_E0. intros; auto. 
+        rewrite H14 in H1; inv H1. rewrite H15 in H2; inv H2; auto.
+      + split. eapply match_traces_E0. intros; auto. 
+        rewrite H14 in H1; inv H1; auto. rewrite H15 in H2; inv H2; auto.
+      + split. eapply match_traces_E0. intros; auto. rewrite H11 in H1; inv H1; auto.
+      + split. eapply match_traces_E0. intros; auto.
+        rewrite H13 in H2; inv H2. rewrite H15 in H4; inv H4; auto.
+      + eapply eval_builtin_args_determ in H1. 2: { eapply H13. } subst.
+        split. eapply external_call_match_traces; eauto.
+        intros. subst. eapply external_call_deterministic in H2. 2:{ eapply H14. }
+        destruct H2; subst; auto.
+      + split. eapply match_traces_E0. intros; auto.
+      + split. eapply match_traces_E0. intros; auto. rewrite H10 in H1; inv H1; auto.
+      + split. eapply match_traces_E0. intros; auto. rewrite H15 in H3; inv H3; auto.
+      + rewrite H13 in H1; inv H1. 
+      + rewrite H12 in H1; inv H1.
+      + split. eapply match_traces_E0. intros; auto.
+      + split. eapply match_traces_E0. intros; auto. rewrite H13 in H1; inv H1; auto.
+        rewrite H14 in H2; inv H2; auto. rewrite H15 in H3; inv H3; auto.
+      + split. eapply match_traces_E0. intros; auto. rewrite H9 in H1; inv H1; auto.
+      + split. eapply match_traces_E0. intros; auto. rewrite H7 in H1; inv H1; auto.
+      + split. eapply external_call_match_traces; eauto.
+        intros; subst. eapply external_call_deterministic in H2. 2:{ eapply H8. }
+        destruct H2; subst; auto.
+      + split. eapply match_traces_E0. intros; auto.
+    - hnf. intros. inv H; auto.
+      eapply ec_trace_length. eapply external_call_spec. eauto.
+      eapply ec_trace_length. eapply external_call_spec. eauto.
+    - intros. inv H. inv H0. rewrite H1 in H. inv H.
+      unfold ge in H2, H3. unfold ge0 in H5, H6.
+      rewrite H5 in H2; inv H2; auto.
+      rewrite H6 in H3; inv H3; auto.
+    - intros. hnf. intros. intro. inv H. inv H0. 
+    - intros. inv H; inv H0. rewrite H1 in H4. inv H4; auto.
+  Qed.
+
+Inductive match_fundef0: fundef -> fundef -> Prop :=
+  | match_fundef0_internal: forall n f,
+      match_fundef0 (Internal f) (Internal (try_swap_nth_func n f))
+  | match_fundef0_external: forall f, match_fundef0 (External f) (External f)
+.
+
 Inductive match_fundef (p: program): fundef -> fundef -> Prop :=
-  (* | match_fundef_same: forall f, match_fundef p f f *)
   | match_fundef_internal: forall n f,
       match_fundef p (Internal f) (Internal (try_swap_nth_func n f))
   | match_fundef_external: forall f, match_fundef p (External f) (External f)
-  .
+.
 
 Lemma match_fundef_refl: forall p f, match_fundef p f f.
 Proof. 
@@ -508,110 +389,60 @@ Qed.
 
 Definition match_varinfo: unit -> unit -> Prop := eq.
 
+
+
+
+
 Inductive match_stackframe: stackframe -> stackframe -> Prop :=
   | match_stackframes_intro:
-      forall f f' sp sp'  ra ra' m c c'
-      (FUNC: f = f') 
+      forall n f f' sp sp' ls ls' m c c'
+      (FUNC: try_swap_nth_func n f = f') 
       (SP: sp = sp')  
-      (RA: ra = ra')  (* TODO: what relation should it be *)
+      (LS: lsagree ls ls')
       (CODE: try_swap_code m c = c'),
-      match_stackframe (Stackframe f sp (Vptr f ra) c)
-                       (Stackframe f' sp' (Vptr f' ra') c')
+      match_stackframe (Stackframe f sp ls c)
+                       (Stackframe f' sp' ls' c')
 .
 
-Lemma match_stack_refl: forall f sp ra c, 
-  match_stackframe (Stackframe f sp (Vptr f ra) c) 
-                   (Stackframe f sp (Vptr f ra) c).
+(* 
+Lemma match_stack_refl: forall f sp rs c, 
+  match_stackframe (Stackframe f sp rs c) 
+                   (Stackframe f sp rs c).
 Proof. 
   intros. eapply match_stackframes_intro; auto. 
   eapply try_swap_at_tail.
-Qed.
+Qed. *)
 
 Definition match_stack := Forall2 match_stackframe.
 
-Lemma match_stack_inv_parent_sp:
-  forall stk stk', match_stack stk stk' -> parent_sp stk = parent_sp stk'.
-Proof. destruct 1; simpl; auto. inv H; auto. Qed. 
-
-Lemma match_stack_inv_parent_ra:
-  forall stk stk', match_stack stk stk' -> parent_ra stk = parent_ra stk'.
-Proof. destruct 1; simpl; auto. inv H; auto. Qed. 
-
-(* try-swap will not swap two inst. one of which contains mem. write *)
 Definition match_mem (m m': mem) := eq m m'.
 
-Section REACHABLE_FROM_INIT.
-  Variable rao: function -> code -> ptrofs -> Prop.
 
-  Inductive reachable (p: program): state -> Prop :=
-    | reachable_initial: forall s, initial_state p s -> reachable p s
-    | reachable_star: forall s1 t s2, 
-        reachable p s1 -> step rao (Genv.globalenv p) s1 t s2 -> reachable p s2 
-  .
-
-  Lemma wf_from_initial: 
-    forall p s, reachable p s -> wf_state (Genv.globalenv p) s.
-  Proof. induction 1. eapply wf_initial; auto. eapply wf_step; eauto. Qed.
-
-  Variable ge: genv.
-  
-  Inductive wf_state_ra: state -> Prop :=
-    | wf_state_ra_state: forall f s fb sp c rs m,
-        Genv.find_funct_ptr ge fb = Some (Internal f) ->
-        load_stack m sp Tptr f.(fn_link_ofs) = Some (parent_sp s) ->
-        load_stack m sp Tptr f.(fn_retaddr_ofs) = Some (parent_ra s) ->
-        wf_state_ra (State s fb sp c rs m)
-    | wf_state_ra_callstate: forall s fb rs m,
-        wf_state_ra (Callstate s fb rs m)
-    | wf_state_ra_returnstate: forall s rs m,
-        wf_state_ra (Returnstate s rs m)
-  .
-
-  (* almost the same as wf_step *)
-  Lemma wf_ra_step:
-  forall S1 t S2, step rao ge S1 t S2 -> wf_state_ra S1 -> wf_state_ra S2.
-  Proof.
-    induction 1; intros WF; inv WF; try (econstructor; now eauto with coqlib).
-    - (* setstack *) 
-      eapply wf_state_ra_state; eauto.
-      Abort.
-
-End REACHABLE_FROM_INIT.
-
-
-Inductive match_states (ge tge: genv): state -> state -> Prop :=
+Inductive match_states: state -> state -> Prop :=
 | match_regular_states: 
-    forall sl sl' fb fb' sp sp' n c c' rs rs' m m'
+    forall sl sl' n_f f f' sp sp' n_c c c' rs rs' m m'
     (STK: match_stack sl sl')
-    (FUNC: fb = fb') (SP: sp = sp')
-    (CODE: try_swap_code n c = c' )
-    (RS: rsagree rs rs') (MEM: match_mem m m')
-    (* (LDSTK: forall f f', Genv.find_funct_ptr ge fb = Some (Internal f) ->
-            Genv.find_funct_ptr tge fb = Some (Internal f') ->
-            load_stack m sp Tptr f.(fn_retaddr_ofs) = Some (parent_ra sl) <->
-            load_stack m' sp Tptr f'.(fn_retaddr_ofs) = Some (parent_ra sl') ) *)
-    (WF: wf_state ge (State sl fb sp c rs m))
-    (WF': wf_state tge (State sl' fb' sp' c' rs' m')),
-    match_states ge tge (State sl fb sp c rs m)
-                        (State sl' fb' sp' c' rs' m')
+    (FUNC: try_swap_nth_func n_f f = f')
+    (SP: sp = sp')
+    (CODE: try_swap_code n_c c = c' )
+    (RS: lsagree rs rs') (MEM: match_mem m m'),
+    match_states (State sl f sp c rs m)
+                 (State sl' f' sp' c' rs' m')
 | match_call_state:
-    forall sl sl' f f' rs rs' m m'
+    forall sl sl' fd fd' rs rs' m m'
     (STK: match_stack sl sl')
-    (FUNC: f = f')        (** TODO: maybe too tough? can we makesure function pointer values are kept during compilation ?  - though not hard to modify to a looser one *)
-    (RS: rsagree rs rs') (MEM: match_mem m m') (** Memory are no way to be different, since we prevented such swapping *)
-    (WF1: wf_state ge (Callstate sl f rs m))
-    (WF2: wf_state tge (Callstate sl' f' rs' m')),
-    match_states ge tge (Callstate sl f rs m)
-                        (Callstate sl' f' rs' m')
+    (FUNC: match_fundef0 fd fd')
+    (RS: lsagree rs rs') 
+    (MEM: match_mem m m'), (** Memory are no way to be different, since we prevented such swapping *)
+    match_states (Callstate sl fd rs m)
+                 (Callstate sl' fd' rs' m')
 | match_return_state:
     forall sl sl' rs rs' m m'
     (STL: match_stack sl sl')
-    (RS: rsagree rs rs')        (** TODO: maybe too tough? do we need a looser definition for regset's match? *)
-    (MEM: match_mem m m')
-    (WF1: wf_state ge (Returnstate sl rs m))
-    (WF2: wf_state tge (Returnstate sl' rs' m')),
-    match_states ge tge (Returnstate sl rs m)
-                        (Returnstate sl' rs' m')
+    (RS: lsagree rs rs') 
+    (MEM: match_mem m m'),
+    match_states (Returnstate sl rs m)
+                 (Returnstate sl' rs' m')
 .
 
 (** Correctness proof of general correctness of instruction scheduling algorithm*)
@@ -639,434 +470,69 @@ Proof.
     - inv H0; apply match_fundef_refl.
 Qed.
 
-
-Definition return_address_offset := Asmgenproof0.return_address_offset.
-Remark return_address_offset_exists:
-  forall f sg ros c, is_tail (Mcall sg ros :: c) (fn_code f) ->
-    exists ofs, return_address_offset f c ofs.
-Proof. intros; eapply Asmgenproof.return_address_exists; eauto. Qed.
-Print Ptrofs.int.
-
-Require Import Integers.
-Lemma return_address_offset_unique: forall f c b tc ofs,
-  return_address_offset f c ofs  -> 
-    Asmgen.transl_code f c b = OK tc ->
-    Z.to_nat (Ptrofs.intval ofs) = length (tc). Abort.
+Require Import Globalenvs.
 
 Section SINGLE_SWAP_CORRECTNESS.
 
   Variable prog: program.
   Variable tprog: program.
-  
-  (* Variable return_address_offset: function -> code -> ptrofs -> Prop.
-  Hypothesis return_address_offset_exists:
-    forall f sg ros c, is_tail (Mcall sg ros :: c) (fn_code f) ->
-      exists ofs, return_address_offset f c ofs. *)
-  
-  (* only try to swap at one pair inside one function *)
-  (* Variable funid: ident. *)
-  (* Variable n: nat. *)
-
-  (* Hypothesis TRANSF: match_prog prog tprog. *)
 
   Hypothesis TRANSF: match_program_gen match_fundef match_varinfo prog prog tprog.
 
   Let ge := Genv.globalenv prog.
   Let tge := Genv.globalenv tprog.
 
-
-  Definition rao_n' (rao: function -> code -> ptrofs -> Prop) (f: function) (c: code): ptrofs -> Prop :=
-    fun ptr => 
-       forall f' c', (exists n, try_swap_nth_func n f = f') ->
-        (exists m, try_swap_code m c = c') -> rao f' c' ptr.
-
-  (* Lemma is_tail_preserved_by_swap:
-    forall sg ros c f n, is_tail (Mcall sg ros :: c) (fn_code f) ->
-      exists m, is_tail (Mcall sg ros :: try_swap_code m c) (fn_code (try_swap_nth_func n f))
-       (* /\ TODO *).
-  Proof.
-    intros sg ros c f n. intros. inv H. 
-    - exists ((n-1)%nat). remember (fn_code f) as fc. destruct (fn_code f). inv H2. inv H. inv H2.
-    induction H.  Admitted. *)
-
-  Let rao_n := rao_n' return_address_offset.
-
-  Lemma rao_n_exists:
-    forall f sg ros c, is_tail (Mcall sg ros :: c) (fn_code f) ->
-      exists ofs, rao_n f c ofs.
-  Proof.
-    intros.
-    (* exploit is_tail_preserved_by_swap; eauto; intros [m]. 
-    clear H; exploit return_address_offset_exists; eauto; intros [ofs].
-    exists ofs. unfold rao_n, rao_n'. intros. destruct H1 as [n']. instantiate (0:= n'). 
-    eexists _. intros.
-    
-    exploit return_address_offset_exists; eauto. intros [ofs].
-    exists ofs.  intros. inv H1; auto. *)
-  Abort.
-
-  Let step' := step return_address_offset. (* target semantics *)
-  Let step := step rao_n. (* source semantics *)
-
-  Let match_states := match_states ge tge.
-
   Lemma symbols_preserved:
-    forall (s: ident), Genv.find_symbol tge s = Genv.find_symbol ge s.
+  forall (s: ident), Genv.find_symbol tge s = Genv.find_symbol ge s.
   Proof (Genv.find_symbol_match TRANSF). 
 
   Lemma senv_preserved:
     Senv.equiv ge tge.
   Proof (Genv.senv_match TRANSF).
 
-  (* Lemma return_address_same: 
-    forall f1 f2, length f1.(fn_code) = length f2.(fn_code) ->
-      forall c1 c2 ofs1 ofs2, return_address_offset f1 c1 ofs1 ->
-        return_address_offset f2 c2 ofs2 -> ofs1 = ofs2.
-  Proof. unfold return_address_offset, Asmgenproof0.return_address_offset. intros.
-    destruct (Asmgen.transf_function f1).   Check Asmgen.transl_code. 
-  Abort. *)
 
-  (* Lemma independ_two_step_match:
-      forall stk1 stk1' f f' sp sp' bb rs1 rs1' m1 m1'
-      s3 s3' i1 i2 t t'
-      (INDEP: happens_before i1 i2 = false)
-      (s1:= State stk1 f sp (i1::i2::bb) rs1 m1)
-      (STEP13: starN step ge 2 s1 t s3)
-      (s1':= State stk1' f' sp' (i2::i1::bb) rs1' m1')
-      (MATCH: match_states s1 s1')
-      (STEP13': starN step ge 2 s1' t' s3'),
-          match_states s3 s3'.
-  Proof.
-      intros.
-      inv STEP13. rename s' into s2. inv H1. inv H3. rename t0 into t2.
-      inv STEP13'. rename s' into s2'. inv H3. inv H5. rename t0 into t1'. rename t4 into t2'.
-(* TODO: use Ltac to reduce proof cost *)
-      assert(B:forall b b1: bool, (if b then b1 else b1) = b1). intros; destruct b; auto.
-      (* 13 branches in total need to reason dependences; others can be discriminated instinctly *) 
-      inv H0; inv H1; unfold happens_before in INDEP; simpl in INDEP; 
-      try rewrite B in INDEP; try discriminate INDEP.
-      (* Mlabel D~> i2 : trivial & discriminated *)
-      (* Mgetstack D~> i2 *)
-        (* Mgetstack D~> Mgetstack *)
-        + inv H2; inv H4. 
-          eapply match_regular_states; eauto; inv MATCH; eauto.
-          eapply try_swap_at_tail. inv MEM.
-          rewrite H11 in H14; inv H14. rewrite H12 in H13; inv H13.
-          eapply rsagree_inv_swap; eauto.
-          unfold happens_before_ww in INDEP; simpl in INDEP.
-          destruct (mreg_eq dst dst0); try discriminate INDEP; auto.
-        (* Mgetstack D~> Mgetparam  *)
-        (* + inv H2; inv H4. 
-          eapply match_regular_states; eauto; inv MATCH; eauto.
-          eapply try_swap_at_tail. inv MEM.
-          erewrite match_stack_inv_parent_sp in H18.
-          rewrite H12 in H15; inv H15. erewrite H18 in H14. inv H14. 
-          intro; unfold Regmap.get. 
-          destruct (mreg_eq r dst); destruct (mreg_eq r dst0); 
-          destruct (mreg_eq r temp_for_parent_frame); subst; simpl; eauto.
-          admit. *)
-        (* Mgetstack D~> Mop  *)
-        + inv H2; inv H4. 
-          eapply match_regular_states; eauto; inv MATCH; eauto.
-          eapply try_swap_at_tail. inv MEM.
-          rewrite H12 in H13; inv H13.
-          admit. 
-        (* Mgetstack D~> Mload  *)
-        + inv H2; inv H4. admit.
-        
-      (* Msetstack D~> i2: trivial & discriminated *)
-        (* Msetstack D~> Mop *)
-        + admit.
-      (* Mgetparam D~> i2: discriminated *)
-      (* Mop D~> i2 *)
-        (* Mop D~> Mgetstack  *)
-        + admit.
-        (* Mop D~> Mset  *)
-        + admit.
-        (* Mop D~> Mgetparam: discriminated *)
-        (* Mop D~> Mop *)
-        + admit.
-        (* Mop D~> Mload *)
-        + admit.
-        (* Mop D~> Mstore *)
-        + admit.
-      (* Mload D~> i2 *)
-        (* Mload D~> Mgetstack *)
-        + admit.
-        (* Mload D~> Mgetparam *)
-        (* Mload D~> Mop *)
-        + admit.
-        (* Mload D~> Mload *)
-        + admit.
-      (* Mstore D~> i2: *)
-        (* Mstore D~> Mop *)
-        + admit.
-      (* Mcall D~> i2: trivial & discriminated *)
-      (* Mtailcall D~> i2: trivial & discriminated *)
-      (* Mbuiltin D~> i2: trivial & discriminated *)
-      (* Mgoto D~> i2: trivial & discriminated *)
-      (* Mcond D~> i2: trivial & discriminated*)
-  Admitted. *)
-
-  Require Import Classical.
-  Lemma regular_state_one_step_match_aux:
+  Lemma regular_state_one_step_match:
   forall stk1 stk1' fb fb' sp sp' c c' rs1 rs1' m1 m1' s2 i t
   (s1:= State stk1 fb sp (i :: c) rs1 m1) (STEP: step ge s1 t s2)
   (s1':= State stk1' fb' sp' (i :: c') rs1' m1') 
   (MATCH: match_states s1 s1'),
-    exists s2', step' tge s1' t s2' 
-        /\ (step' tge s1' t s2' -> match_states s2 s2'). (* note: written in this way only to reduce proof load *)
-  Proof.
-    intros. inv MATCH. eapply wf_step in STEP as WF1; auto.
-    inv STEP; eapply try_swap_head_not_change in CODE; destruct CODE as [n'].
-    (* Mlabel *)
-    eexists (State _ _ _ _ _ _); split. eapply exec_Mlabel.
-    intros; eapply match_regular_states; eauto. eapply wf_step; eauto.
-    (* Mgetstack *)
-    eexists (State _ _ _ _ _ _); split. eapply exec_Mgetstack. inv MEM. eapply H8.
-    intros; eapply match_regular_states; eauto.
-    eapply rsagree_inv_update; eauto. eapply wf_step; eauto.
-    (* Msetstack *)
-    eexists (State _ _ _ _ _ _); split.
-    eapply exec_Msetstack. specialize (RS src); unfold Regmap.get in RS. rewrite <- RS.
-    inv MEM. eapply H8. eauto. intros; eapply match_regular_states; eauto.
-    eapply rsagree_inv_undef_regs_destroyed; eauto. reflexivity.
-    eapply wf_step; eauto.
-    (* Mgetparam *)
-    eapply Genv.find_funct_ptr_match with 
-          (match_fundef:=match_fundef) (match_varinfo:=match_varinfo) in H8.
-    2: { eapply TRANSF. } destruct H8 as [cunit [tf [? [MF]]]].
-    inv MF; eexists (State _ _ _ _ _ _); split.
-    eapply match_stack_inv_parent_sp in STK. eapply exec_Mgetparam; eauto; erewrite <- STK; inv MEM; eauto.
-    intros. eapply match_regular_states; eauto. repeat eapply rsagree_inv_update; eauto. eapply wf_step; eauto.
-    (* Mop *)
-    eexists (State _ _ _ _ _ _); split.
-    eapply exec_Mop; eauto. erewrite <- rsagree_inv_mreg_list; eauto.
-    erewrite <- eval_operation_preserved. inv MEM. eexact H8. 
-    symmetry; eapply symbols_preserved. intros; eapply match_regular_states; eauto. 
-    eapply rsagree_inv_update; eapply rsagree_inv_undef_regs_destroyed; eauto.
-    eapply wf_step; eauto.
-    (* Mload *)
-    eexists (State _ _ _ _ _ _); split.
-    eapply exec_Mload; inv MEM; eauto. erewrite rsagree_inv_mreg_list; eauto.
-    erewrite eval_addressing_preserved; eauto. eapply symbols_preserved.
-    eapply rsagree_symmetric; auto. intros; eapply match_regular_states; eauto.
-    eapply rsagree_inv_update; eapply rsagree_inv_undef_regs_destroyed; eauto.
-    eapply wf_step; eauto.
-    (* Mstore *)
-    eexists (State _ _ _ _ _ _); split.
-    eapply exec_Mstore; inv MEM. erewrite rsagree_inv_mreg_list; eauto.
-    erewrite eval_addressing_preserved; eauto. eapply symbols_preserved.
-    eapply rsagree_symmetric; eauto. specialize (RS src); unfold Regmap.get in RS.
-    erewrite <- RS. eexact H9.
-    2: { intros; eapply match_regular_states; eauto. 
-    eapply rsagree_inv_undef_regs_destroyed; eauto. reflexivity. eapply wf_step; eauto. }
-    eauto.
-    (* Mcall *)
-    erewrite find_function_ptr_genv_irrelevent with (ge2:=tge) in H8; eauto.
-    2: { symmetry; eapply symbols_preserved. }
-    erewrite rsagree_inv_find_function_ptr in H8; eauto.
-    pose proof H9 as H9'.
-    eapply Genv.find_funct_ptr_match with 
-          (match_fundef:=match_fundef) (match_varinfo:=match_varinfo) in H9.
-    2: { eapply TRANSF. } destruct H9 as [cunit [tf [? [MF]]]].
-    assert (wf' := WF').
-    inv WF'. fold tge in H0; erewrite CODE in H0; inv H0. eauto.
-    exploit return_address_offset_exists; eauto; intros [ra'].
-    inv MF; eexists (Callstate _ _ _ _); split.
-    eapply exec_Mcall with (ra:=ra'); eauto. intros; eapply match_call_state; eauto. 
-      eapply Forall2_cons; eauto. eapply match_stackframes_intro; eauto.
-      admit. (* TODO: an unavoidable hard reasoning *)
-      eapply wf_step; eauto.
+    exists s2', step tge s1' t s2' 
+        /\ match_states s2 s2'. (* note: written in this way only to reduce proof load *)
+  Proof. Admitted.
 
-    (* Mtailcall *)
-    erewrite find_function_ptr_genv_irrelevent with (ge2:=tge) in H8; eauto.
-    2: { symmetry; eapply symbols_preserved. }
-    erewrite rsagree_inv_find_function_ptr in H8; eauto.
-    pose proof H9 as H9'.
-    eapply Genv.find_funct_ptr_match with 
-          (match_fundef:=match_fundef) (match_varinfo:=match_varinfo) in H9.
-    2: { eapply TRANSF. } destruct H9 as [cunit [tf [? [MF]]]].
-    inv MEM. inv MF; eexists (Callstate _ _ _ _); split.
-    eapply exec_Mtailcall; simpl; eauto. 
-    eapply match_stack_inv_parent_sp in STK; erewrite <- STK; eauto.
-    eapply match_stack_inv_parent_ra in STK; erewrite <- STK; eauto.
-    intros. eapply match_call_state; eauto. reflexivity. eapply wf_step; eauto.
-    (* Mbuiltin *)
-    eexists (State _ _ _ _ _ _); split.
-    eapply exec_Mbuiltin; inv MEM.
-    eapply rsagree_inv_eval_builtin_args with (rs:=rs1) in H8. 2: { eauto. }
-    eapply eval_builtin_args_preserved. eapply symbols_preserved. eauto.
-    eapply extcall_genv_irrelevent; eauto. eapply senv_preserved. eauto.
-    intros; eapply match_regular_states; eauto.
-    eapply rsagree_inv_set_res; eapply rsagree_inv_undef_regs_destroyed; auto. reflexivity.
-    eapply wf_step; eauto.
 
-    (* Mgoto *)
-    eapply Genv.find_funct_ptr_match with 
-          (match_fundef:=match_fundef) (match_varinfo:=match_varinfo) in H8.
-    2: { eapply TRANSF. } destruct H8 as [cunit [tf [? [MF]]]].
-    inv MF. pose proof (find_label_try_swap lbl (fn_code f)) c'0 n0 H9. destruct H as [nn].
-    eexists (State _ _ _ _ _ _); split. eapply exec_Mgoto; eauto.
-    intros. eapply match_regular_states; eauto. eapply wf_step; eauto.
+  Lemma independ_two_step_match:
+      forall stk1 stk1' f f' sp sp' bb rs1 rs1' m1 m1' s3 i1 i2 t t'
+      (INDEP: happens_before i1 i2 = false)
+      (s1:= State stk1 f sp (i1::i2::bb) rs1 m1)
+      (STEP13: starN step ge 2 s1 t s3)
+      (s1':= State stk1' f' sp' (i2::i1::bb) rs1' m1')
+      (MAT: match_states s1 s1'),
+      exists s3',
+      starN step ge 2 s1' t' s3' /\ match_states s3 s3'.
+  Proof. Admitted.
 
-    (* Mcond_true *)
-    eapply Genv.find_funct_ptr_match with 
-          (match_fundef:=match_fundef) (match_varinfo:=match_varinfo) in H9.
-    2: { eapply TRANSF. } destruct H9 as [cunit [tf [? [MF]]]].
-    inv MF. pose proof (find_label_try_swap lbl (fn_code f)) c'0 n0 H10. destruct H as [nn].
-    eexists (State _ _ _ _ _ _); split. eapply exec_Mcond_true; eauto.
-    inv MEM. erewrite <- rsagree_inv_mreg_list; eauto.
-    intros. eapply match_regular_states; eauto. eapply wf_step; eauto.
-
-    (* Mcond_false *)
-    eexists (State _ _ _ _ _ _); split. eapply exec_Mcond_false; eauto.
-    inv MEM. erewrite <- rsagree_inv_mreg_list; eauto.
-    intros. eapply match_regular_states; eauto. eapply wf_step; eauto.
-    (* Mcond_jumptable *)
-    eapply Genv.find_funct_ptr_match with 
-          (match_fundef:=match_fundef) (match_varinfo:=match_varinfo) in H10.
-    2: { eapply TRANSF. } destruct H10 as [cunit [tf [? [MF]]]].
-    inv MF. pose proof (find_label_try_swap lbl (fn_code f)) c'0 n1 H11. destruct H as [nn].
-    eexists (State _ _ _ _ _ _); split. eapply exec_Mjumptable; eauto.
-    rewrite <- H8; symmetry; apply RS.
-    intros. eapply match_regular_states; eauto. eapply rsagree_inv_undef_regs_destroyed; eauto.
-    eapply wf_step; eauto.
-    (* Mreturn *) 
-    eapply Genv.find_funct_ptr_match with 
-          (match_fundef:=match_fundef) (match_varinfo:=match_varinfo) in H8.
-    2: { eapply TRANSF. } destruct H8 as [cunit [tf [? [MF]]]]. inv MEM.
-
-    inv MF; eauto; eexists (Returnstate stk1' _ _); split.
-      eapply exec_Mreturn; eauto.
-      erewrite <- match_stack_inv_parent_sp; eauto.
-      erewrite <- match_stack_inv_parent_ra; eauto.
-      intros; eapply match_return_state; eauto. reflexivity. eapply wf_step; eauto.
-Admitted.
-
-  Lemma regular_state_one_step_match:
-  forall stk1 stk1' f f' sp sp' c c' rs1 rs1' m1 m1' s2 i t
-  (s1:= State stk1 f sp (i :: c) rs1 m1) (STEP: step ge s1 t s2)
-  (s1':= State stk1' f' sp' (i :: c') rs1' m1') (MATCH: match_states s1 s1'),
-    exists s2', step' tge s1' t s2' 
-      /\ match_states s2 s2'.
-  Proof. intros. edestruct regular_state_one_step_match_aux; eauto. destruct H; eexists x; split; eauto. Qed.
-
-  Let tplus:= Plus (semantics return_address_offset tprog).
-  Let tEventually:= Eventually (semantics rao_n prog).
-  
-  Lemma simulation:
-  forall s1 t s1', step ge s1 t s1' ->
-  forall s2, match_states s1 s2 ->
-    exists n s2',
-      tplus s2 t s2' /\ tEventually n s1' (fun s1'' => match_states s1'' s2').
-  Proof. 
-    intros. inv H0; eapply wf_step in H as WF1'; eauto.  
-    (* State *)
-    -  destruct c as [ | i1]. inv H. destruct c as [|i2 c].
-      (* take one step *)
-      { exists 0%nat. inv MEM.
-        edestruct regular_state_one_step_match. eapply H. eapply match_regular_states; eauto.
-        eapply try_swap_at_tail. instantiate (1:=m'); unfold match_mem; auto. 
-        erewrite <- try_swap_singleton; eauto. 
-        exists x. split. 
-        eapply plus_one. unfold try_swap_code. erewrite try_swap_singleton. eapply H0.
-        eapply eventually_now; auto. destruct H0; auto. }
-      (* safe swap, match after two step *)
-      { destruct n.
-        (* try-swap now *)
-        + simpl. remember (i1 D~> i2) as INDEP. 
-          symmetry in HeqINDEP. destruct INDEP.
-          (* swap failed, take two independent steps, from previous lemma  *)
-          { exists 0%nat. inv MEM.
-            edestruct regular_state_one_step_match. eapply H. eapply match_regular_states; eauto.
-            eapply try_swap_at_tail. instantiate (1:=m'); unfold match_mem; auto.
-            simpl in WF'; rewrite HeqINDEP in WF'; auto. 
-            destruct H0.
-            exists x. split. eapply plus_one. unfold try_swap_code. eapply H0.
-            eapply eventually_now; auto.  
-          }
-          (* swap succeeded, take two independent steps, from previous lemma  *)
-          { exists 1%nat.
-            admit.
-          }
-        (* try-swap later, take one step *)
-        + exists 0%nat. simpl in *.
-          edestruct regular_state_one_step_match. eapply H. eapply match_regular_states; eauto.
-          instantiate(1:=Datatypes.S n). simpl. eapply eq_refl. unfold match_mem; auto.
-          destruct H0.
-          exists x. split. eapply plus_one. eapply H0.  
-          eapply eventually_now; auto.  
-      }
-      (* Callstate: one-step-match *)
-    - exists 0%nat. inv MEM. inv H. 
-      (* call internal *)
-      + eapply Genv.find_funct_ptr_match with 
-          (match_fundef:=match_fundef) (match_varinfo:=match_varinfo) in H4.
-        2: { eapply TRANSF. }
-        destruct H4 as [cunit [tf [? [MF]]]].
-        inv MF; eexists (State _ _ _ _ _ _ ).
-        (* { split. eapply plus_one. eapply exec_function_internal; eauto. 
-          eapply match_stack_inv_parent_sp in STK. erewrite <- STK; eauto.
-          erewrite <- match_stack_inv_parent_ra; eauto.
-          eapply eventually_now. eapply match_regular_states; eauto.
-          eapply try_swap_at_tail. eapply rsagree_inv_undef_regs_destroyed; eauto.
-          unfold match_mem; auto. eapply wf_step; eauto. eapply exec_function_internal; eauto.
-          eapply match_stack_inv_parent_sp in STK. erewrite <- STK; eauto.
-          erewrite <- match_stack_inv_parent_ra; eauto.    } *)
-        { split. eapply plus_one. eapply exec_function_internal; eauto. 
-          eapply match_stack_inv_parent_sp in STK. erewrite <- STK; eauto.
-          erewrite <- match_stack_inv_parent_ra; eauto. 
-          eapply eventually_now. eapply match_regular_states; eauto.
-          simpl; eauto. eapply rsagree_inv_undef_regs_destroyed; eauto.
-          unfold match_mem; auto. eapply wf_step; eauto. eapply exec_function_internal; eauto.
-          eapply match_stack_inv_parent_sp in STK. erewrite <- STK; eauto.
-          erewrite <- match_stack_inv_parent_ra; eauto. }
-      (* call external *)
-      + eapply Genv.find_funct_ptr_match with 
-          (match_fundef:=match_fundef) (match_varinfo:=match_varinfo) in H4.
-        2: { eapply TRANSF. }
-        destruct H4 as [cunit [tf [? [MF]]]]. inv MF.
-        eexists (Returnstate _ _ _). split.
-        eapply plus_one. eapply exec_function_external; eauto.
-        eapply match_stack_inv_parent_sp in STK. erewrite <- STK; eauto.
-        eapply rsagree_inv_extcall_arguments; eauto.
-        eapply extcall_genv_irrelevent in H8. eapply H8.
-        eapply senv_preserved.
-        eapply eventually_now. eapply match_return_state; eauto. 
-        eapply rsagree_inv_set_pair; eapply rsagree_inv_undef_caller_save_regs; eauto. 
-        hnf; auto. eapply wf_step; eauto. eapply exec_function_external; eauto.
-        eapply match_stack_inv_parent_sp in STK. erewrite <- STK; eauto.
-        eapply rsagree_inv_extcall_arguments; eauto.
-        eapply extcall_genv_irrelevent in H8. eapply H8.
-        eapply senv_preserved.
-    (* Returnstate: one-step-match *)
-    - exists 0%nat. inv H. inv STL. inv H1. eexists (State _ _ _ _ _ _ ). split.
-      + apply plus_one. eapply exec_return.
-      + eapply eventually_now. eapply match_regular_states; eauto.
-        eapply wf_step; eauto; eapply exec_return; eauto. 
-  Admitted.
-
-  Lemma transf_initial_states_aux:
-    forall st1, initial_state prog st1 ->
-    exists st2, initial_state tprog st2 
-      /\ (initial_state tprog st2 -> match_states st1 st2).
-  Proof. 
-      intros. eapply wf_initial in H as ?. inv H.
-      exists (Callstate [] fb (Regmap.init Vundef) m0).
-      split.
-      - apply initial_state_intro.
-          apply (Genv.init_mem_match TRANSF); trivial. 
-          rewrite (match_program_main TRANSF).
-          rewrite symbols_preserved; auto. 
-      - intros. apply match_call_state; auto. apply Forall2_nil. 
-        intro; auto. hnf; auto. eapply wf_initial; auto. 
-  Qed.
 
   Lemma transf_initial_states:
     forall st1, initial_state prog st1 ->
     exists st2, initial_state tprog st2 /\ match_states st1 st2.
-  Proof. intros. edestruct transf_initial_states_aux; intros; eauto. destruct H0; eauto. Qed.
+  Proof.
+    intros. inv H.
+    eapply (Genv.find_funct_ptr_match TRANSF) in H2; eauto.
+    destruct H2 as [cu [tf [? []]]]. inv H2.
+    - exists (Callstate [] (Internal ((try_swap_nth_func n f0))) (Locmap.init Vundef) m0).
+      split. eapply initial_state_intro; eauto.
+      eapply (Genv.init_mem_match TRANSF); trivial. 
+      rewrite (match_program_main TRANSF); rewrite symbols_preserved; auto.
+      eapply match_call_state; eauto. eapply Forall2_nil.
+      eapply match_fundef0_internal. eapply lsagree_refl. reflexivity.
+    - exists (Callstate [] (External f0)  (Locmap.init Vundef) m0).
+      split. eapply initial_state_intro; eauto.
+      eapply (Genv.init_mem_match TRANSF); trivial. 
+      rewrite (match_program_main TRANSF); rewrite symbols_preserved; auto.
+      eapply match_call_state; eauto. eapply Forall2_nil.
+      eapply match_fundef0_external. eapply lsagree_refl. reflexivity.
+  Qed.
 
   Lemma transf_final_states:
     forall st1 st2 r,
@@ -1074,155 +540,7 @@ Admitted.
   Proof. 
     intros. inv H0. inv H. inv STL.
     eapply final_state_intro.
-    eapply H1. specialize (RS r0). unfold Regmap.get in RS.
-    erewrite <- RS. trivial.
-  Qed.
-  
-  Theorem forward_simulation_transformed:
-  forward_simulation (Mach.semantics rao_n prog) 
-                     (Mach.semantics return_address_offset tprog).
-  Proof.
-    eapply forward_simulation_eventually_plus.
-    - apply senv_preserved.
-    - apply transf_initial_states.
-    - apply transf_final_states.
-    - apply simulation.
-  Qed.
-
-End SINGLE_SWAP_CORRECTNESS.
-
-
-
-(* Real Instruction Scheduling Correctness *)
-
-Definition transf_function (f: Mach.function) : res Mach.function.
-Admitted.
-
-Definition transf_fundef (f: Mach.fundef) : res Mach.fundef :=
-  AST.transf_partial_fundef transf_function f.
-
-Definition transf_program (p: Mach.program): res Mach.program :=
-  transform_partial_program transf_fundef p.
-
-Definition match_prog_real (p: Mach.program) (tp: Mach.program) :=
-  match_program (fun ctx f tf => transf_fundef f = OK tf) eq p tp.
-
-Lemma transf_program_match_real:
-  forall p tp, transf_program p = OK tp -> match_prog_real p tp.
-Proof.
-  intros. eapply match_transform_partial_program; eauto.
-Qed.
-
-Section SCHEDULING_CORRECTNESS.
-
-  Variable prog: program.
-  Variable tprog: program.
-
-  Hypothesis TRANSF: match_prog_real prog tprog.
-
-  Lemma to_sequence_transf (p: program):
-    exists lfd, 
-      transf_program p = transf_program_sequence lfd p.
-  Proof. 
-    unfold match_prog, match_program in TRANSF.
-    unfold match_program_gen in TRANSF.
-    destruct TRANSF as [ TRANSF_ [? ?]]; clear TRANSF.
-    unfold transf_program, transform_partial_program .
-    unfold transform_partial_program2. 
-
   Admitted.
 
-
-  Variable return_address_offset: function -> code -> ptrofs -> Prop.
   
-  (* only try to swap at one pair inside one function *)
-  Variable funid: ident.
-  Variable ln: list nat.
-  (* Hypothesis TRANSF: match_prog prog tprog. *)
-  (* Hypothesis TRANSF_PROG: transf_program_try_swap_nth_in_one funid ln prog = OK tprog. *)
-  Let step := step return_address_offset.
-
-  Let ge := Genv.globalenv prog.
-  Let tge := Genv.globalenv tprog.
-(* 
-  Let transf_fun := (fun i f => if ident_eq i funid then transf_fundef_try_swap_nth n f else OK f).
-  Let transf_var := (fun (i: ident) (v:unit) => OK v). *)
-
-End SCHEDULING_CORRECTNESS.
-
-Require Import Errors.
-Open Scope error_monad_scope.
-Import ListNotations.
-Open Scope list_scope. 
-
-Fixpoint list2bbs (l: list instruction): list (list instruction) :=
-  match l with
-  (* termination *)
-  | Mgoto lb :: l' =>  [Mgoto lb] :: list2bbs l'
-  | Mcond con rs lb :: l' => [Mcond con rs lb] :: list2bbs l' 
-  | Mjumptable r lbs :: l' => [Mjumptable r lbs] :: list2bbs l'
-  | Mreturn :: l' => [Mreturn] :: list2bbs l' 
-  (* non-termination *) 
-  | inst :: l' => 
-      match list2bbs l' with
-      | (Mlabel lb :: l'') :: ll => [inst] :: (Mlabel lb :: l'') :: ll
-      | l'' :: ll  => (inst :: l'') :: ll
-      | nil => [ [inst] ]
-      end 
-  | nil => nil
-  end. 
-
-Fixpoint bbs2list (ll: list (list instruction)): list instruction :=
-  match ll with 
-  | l :: ll' => l ++ bbs2list ll'
-  | nil => nil
-  end.
-
-Lemma list2bbs_recover: forall l, bbs2list (list2bbs l) = l.
-Proof. 
-  induction l. simpl; trivial.
-Admitted.
-
-
-
-
-(* Definition transf_code:= list2bbs.
-
-Definition transf_function (f: Mach.function) : res function :=
-  OK ( 
-    let code' := transf_code(Mach.fn_code f) in
-    (mkfunction (Mach.fn_sig f) (Mach.fn_stacksize f) 
-      (code') (Mach.fn_link_ofs f) (Mach.fn_retaddr_ofs f) )
-  ). 
-
-Definition transf_fundef (f: Mach.fundef) : res fundef :=
-    AST.transf_partial_fundef transf_function f.
-
-Definition transf_program (p: Mach.program) : res program :=
-    transform_partial_program transf_fundef p. *)
-
-
-
-    Section GENV_2_6.
-
-    Variable A B V W: Type.
-    Variable transf_fun: ident -> A -> res B.
-    Variable transf_var: ident -> V -> res W.
-    Variable p: AST.program A V.
-    Variable p': AST.program B W.
-    Hypothesis transf_OK:
-      transform_partial_program2 transf_fun transf_var p = OK p'.
-    
-    (* Remark transf_augment_OK:
-      transform_partial_augment_program transf_fun transf_var nil p.(prog_main) p = OK p'.
-    Proof.
-      rewrite <- transf_OK. symmetry. apply transform_partial_program2_augment.
-    Qed. *)
-    End GENV_2_6.
-    
-
-
-
-
-
-
+End SINGLE_SWAP_CORRECTNESS.
